

Appendix A

Proofs of Theorems

A.1 Proofs of Theorems 1-3 in Section 2

To simplify the notations, let $T_i = \sqrt{n}(\hat{\beta}_i - \beta_i)$, $T_i^* = \sqrt{n}(\beta_i^* - \hat{\beta}_i)$, $d_{\max} = \beta_{\max} - \max_{i \notin H} \beta_i$ and $V = (V_1, \dots, V_k)$ where $V_i = \hat{\beta}_{\max} - \beta_{\max} - \hat{\beta}_i + \beta_i$. We start with two lemmas that are essential for the proof of Theorem 1.

Lemma 1.1: *Under Assumption 1.1, we have*

$$\sup_{x \in R} |P(\sqrt{n}(\hat{\beta}_{\max} - \beta_{\max}) \leq x) - P(\max_{i \in H} T_i \leq x)| \rightarrow 0$$

as $n \rightarrow \infty$.

Proof: For any $x \in R$, we have

$$\begin{aligned} & |P(\sqrt{n}(\hat{\beta}_{\max} - \beta_{\max}) \leq x) - P(\max_{i \in H} T_i \leq x)| \\ &= |P(\max_{i \in H} T_i \leq x, T_j \leq x + \sqrt{n}(\beta_{\max} - \beta_j), j \notin H) - P(\max_{i \in H} T_i \leq x)| \quad (\text{A.1}) \\ &\leq 1 - P(\max_{i \notin H} T_i \leq x + \sqrt{n}d_{\max}). \end{aligned}$$

For any $x \in R$, by Assumption 1.1, we have $1 - P(\max_{i \notin H} T_i \leq x + \sqrt{n}d_{\max}) \rightarrow 0$, so

$$|P(\sqrt{n}(\hat{\beta}_{\max} - \beta_{\max}) \leq x) - P(\max_{i \in H} T_i \leq x)| \rightarrow 0$$

as $n \rightarrow \infty$. The result follows naturally from the property of the cdf. \square

Lemma 1.2: *Under Assumptions 1.1 and 1.2, for $0 < r < 0.5$, we have*

$$\sup_{x \in R} |P^*(\sqrt{n}(\beta_{\max, \text{modified}}^* - \hat{\beta}_{\max}) \leq x) - P(\max_{i \in H} T_i \leq x)| \rightarrow 0$$

as $n \rightarrow \infty$, in probability w.r.t. P .

Proof: Similar to the proof in Lemma 1.1, we have

$$\begin{aligned} & |P^*(\sqrt{n}(\beta_{\max, \text{modified}}^* - \hat{\beta}_{\max}) \leq x) - P^*(T_i^* \leq x + n^r V_i, i \in H)| \\ &= |P^*(T_i^* \leq x + n^r V_i, i \in H, T_j^* \leq x + n^r V_j + n^r(\beta_{\max} - \beta_j), j \notin H) - P^*(T_i^* \leq x + n^r V_i, i \in H)| \\ &\leq 1 - P^*(T_j^* \leq x + n^r d_{\max} - n^r \|V\|_{\infty}, j \notin H). \end{aligned} \quad (\text{A.2})$$

When $0 < r < 0.5$, by Assumptions 1.1 and 1.2, we have $n^r \|V\|_\infty \rightarrow 0$ in probability and

$$1 - P^*(T_j^* \leq x + n^r d_{\max} - n^r \|V\|_\infty, j \notin H) \rightarrow 0$$

in probability. By Assumptions 1.1 and 1.2, we have $|P^*(T_i^* \leq x + n^r V_i) - P(\max_{i \in H} T_i \leq x)| \rightarrow 0$ in probability so

$$|P^*(\sqrt{n}(\beta_{\max, \text{modified}}^* - \hat{\beta}_{\max}) \leq x) - P(\max_{i \in H} T_i \leq x)| \rightarrow 0$$

in probability w.r.t P . The result is naturally followed by the property of cdf. \square

Proof of Theorem 1: It follows from Lemmas 1.1 and 1.2. \square

Proof of Corollary 1.1: The result is true, because $\sqrt{n}(\beta_s - \beta_{\max}) \rightarrow 0$ in probability. Otherwise, by the definition of β_s , the probability of the event, $\max_{i \notin H} \hat{\beta}_i \geq \max_{i \in H} \hat{\beta}_i$, will not go to 0 asymptotically, which violates the consistency implied in Assumption 1.1. \square

Lemma 2.1: Under Assumptions 1.1 and 2.1, we have

$$|E[\sqrt{n}(\hat{\beta}_{\max} - \beta_{\max})] - E[\max_{i \in H} T_i]| \rightarrow 0$$

as $n \rightarrow \infty$.

Proof: By Assumption 2.1, we have $E[\max_{i \in H} T_i]^2 \leq E[\max_{i \in H} T_i^2] \leq \sum_{i \in H} E T_i^2 < \infty$ and similarly $E[\max_{i \notin H} T_i]^2 < \infty$ uniformly in n , so

$$\begin{aligned} E[\sqrt{n}(\hat{\beta}_{\max} - \beta_{\max})]^2 &= E[\max_{i \in H} T_i + \max(0, \max_{j \notin H} \sqrt{n}(\hat{\beta}_j - \max_{i \in H} \hat{\beta}_i))]^2 \\ &\leq 2\{E[\max_{i \in H} T_i]^2 + E[\max(0, \max_{j \notin H} (T_j - \max_{i \in H} T_i))]^2\} < \infty \end{aligned} \quad (\text{A.3})$$

uniformly in n . By Assumption 1.1 and Lemma 1.1, the lemma follows from the uniform integrability for $\sqrt{n}(\hat{\beta}_{\max} - \beta_{\max})$; i.e.

$$\begin{aligned} &E|\sqrt{n}(\hat{\beta}_{\max} - \beta_{\max})|I_{|\sqrt{n}(\hat{\beta}_{\max} - \beta_{\max})| > c} \\ &\leq [E[\sqrt{n}(\hat{\beta}_{\max} - \beta_{\max})]^2 P(\sqrt{n}(\hat{\beta}_{\max} - \beta_{\max}) > c)]^{1/2} \rightarrow 0 \end{aligned} \quad (\text{A.4})$$

uniformly in n as $c \rightarrow \infty$. \square

Lemma 2.2: Under Assumptions 1.1, 1.2, and 2.2, and for any $0 < r < 0.5$, we have

$$E^*[\sqrt{n}(\beta_{\max, \text{modified}}^* - \hat{\beta}_{\max})] - E \max_{i \in H} T_i \rightarrow 0$$

as $n \rightarrow \infty$, in probability w.r.t P .

Proof: Similar to the proof in Lemma 2.1, by Assumption 2.2, we have $E^*[\max_{i \in H} T_i^* - n^r V_i]^2 < \infty$ and $E^*[\max_{i \notin H} T_i^* - n^r V_i]^2 < \infty$ uniformly in n in probability, and then

$$\begin{aligned} &E^*[\sqrt{n}(\beta_{\max, \text{modified}}^* - \hat{\beta}_{\max})]^2 \\ &= E^*[\max_{i \in H} (T_i^* - n^r V_i) + \max(0, \max_{j \notin H} (T_j^* - n^r V_j - \max_{i \in H} (T_i^* - n^r V_i)))]^2 \\ &\leq 2\{E^*[\max_{i \in H} (T_i^* - n^r V_i)]^2 + E^*[\max(0, \max_{j \notin H} (T_j^* - n^r V_j - \max_{i \in H} (T_i^* - n^r V_i)))]^2\} < \infty \end{aligned} \quad (\text{A.5})$$

uniformly in n . The lemma then follows from Assumptions 1.1, 1.2 and Lemma 1.2 with the similar argument of uniform integrability in Lemma 2.1 but for $\sqrt{n}(\beta_{\max, \text{modified}}^* - \hat{\beta}_{\max})$.

Proof of Theorem 2: By Lemmas 2.1 and 2.2, the result follows. \square

Proof of Corollary 2.1: It follows from Theorem 2 and similar arguments of the uniform integrability in Lemma 2.2 but for $E^*[\sqrt{n}(\beta_{\max, \text{modified}}^* - \hat{\beta}_{\max})]$. \square

Proof of Theorem 3: By definition, we have

$$\begin{aligned} & E[\hat{\beta}_{\max, \text{reduced}, 1}(r) - \beta_i]^2 \\ &= E[\hat{\beta}_{\max, \text{reduced}, 1}(r) - \beta_{\max}]^2 + (\beta_{\max} - \beta_i)^2 + 2E[\hat{\beta}_{\max, \text{reduced}, 1}(r) - \beta_{\max}](\beta_{\max} - \beta_i) \end{aligned} \quad (\text{A.6})$$

By Assumptions in Corollary 2.1, we have $E[\hat{\beta}_{\max, \text{reduced}, 1}(r) - \beta_{\max}] = o(1)$, which implies the desired result. \square

A.2 Proofs of Theorems 4-5 in Section 3

To simplify the notation, we let $K + d = \{c : \text{distance}(c, K) \leq d\} \cap D$, $\overline{K + d}$ denote the complement of the set $K + d$, $(K + d) - K = (K + d) \cap \overline{K}$, $G_n(c) = \sqrt{n}(\hat{\beta}(c) - \beta(c))$ and $G_n^*(c) = \sqrt{n}(\beta^*(c) - \hat{\beta}(c))$. By Assumption 4.3, we know γ_{\max} is achievable and K is a compact set, so all the above notations are well defined.

Lemma 4.1: Under Assumptions 4.1 and 4.3, for any $x \in R$,

$$\lim_{n \rightarrow \infty} P(\sqrt{n}(\hat{\gamma}_{\max} - \gamma_{\max}) \leq x) = P(\sup_{c \in K} G(c) \leq x).$$

Proof: By definition, we have

$$\begin{aligned} & P(\sqrt{n}(\hat{\gamma}_{\max} - \gamma_{\max}) \leq x) \\ &= P(\sqrt{n} \sup_{c \in D} (\hat{\beta}(c) - \beta(c) + \beta(c) - \gamma_{\max}) \leq x) \\ &= P(\max(\sup_{c \in K+d} (G_n(c) + \sqrt{n}(\beta(c) - \gamma_{\max})), \sup_{c \in \overline{K+d}} (G_n(c) + \sqrt{n}(\beta(c) - \gamma_{\max}))) \leq x). \end{aligned} \quad (\text{A.7})$$

From Assumption 4.3, $\sqrt{n}(\beta(c) - \gamma_{\max})$ converges to negative infinity uniformly in $\overline{K + d}$, so by Assumption 4.1, we have

$$\sup_{c \in \overline{K+d}} (G_n(c) + \sqrt{n}(\beta(c) - \gamma_{\max})) \rightarrow -\infty$$

in probability. Therefore, the right hand side of (A.7) is asymptotically equivalent to

$$P(\sup_{c \in K+d} (G_n(c) + \sqrt{n}(\beta(c) - \gamma_{\max})) \leq x) \quad (\text{A.8})$$

for any given d . Since for $c \in K$, $\beta(c) = \gamma_{\max}$, and for $c \in (K + d) - K$, $\beta(c) < \gamma_{\max}$, we have the following inequality.

$$P(\sup_{c \in K+d} G_n(c) \leq x) \leq (\text{A.8}) \leq P(\sup_{c \in K} G_n(c) \leq x). \quad (\text{A.9})$$

Let $n \rightarrow \infty$, under Assumption 4.2, we have

$$P(\sup_{c \in K+d} G(c) \leq x) \leq \liminf (\text{A.8}) \leq \limsup (\text{A.8}) \leq P(\sup_{c \in K} G(c) \leq x). \quad (\text{A.10})$$

Let $L_n(x) = P(\sqrt{n}(\hat{\gamma}_{\max} - \gamma_{\max}) \leq x)$ and recall that $L_n(x)$ is asymptotically equivalent to (A.8). Therefore, for any $d > 0$, we have

$$P(\sup_{c \in K+d} G(c) \leq x) \leq \liminf L_n(x) \leq \limsup L_n(x) \leq P(\sup_{c \in K} G(c) \leq x). \quad (\text{A.11})$$

Under Assumptions 4.1 and 4.3, $\lim_{d \rightarrow 0} \sup_{c \in K+d} G(c) = \sup_{c \in K} G(c)$, in probability. Let $d \rightarrow 0$ in (A.11), we prove the desired result. \square

Lemma 4.2: *Under Assumptions 4.1, 4.2 and 4.3 and $0 < r < 0.5$, for any $x \in R$,*

$$\lim_{n \rightarrow \infty} P^*(\sqrt{n}(\gamma_{\max, \text{modified}}^* - \hat{\gamma}_{\max}) \leq x) = P(\sup_{c \in K} G(c) \leq x)$$

in probability.

Proof: With similar arguments as those in the proof of Lemma 4.1, we have

$$\begin{aligned} & P^*(\sqrt{n}(\gamma_{\max, \text{modified}}^* - \hat{\gamma}_{\max}) \leq x) \\ &= P^*(\sup_{c \in D} (G_n^*(c) - n^r \sup_{b \in D} [\hat{\beta}(b) - \hat{\beta}(c)]) \leq x) \\ &= P^*(\sqrt{n} \max(\sup_{c \in K+d} (G_n^*(c) - n^r \sup_{b \in D} (\hat{\beta}(b) - \hat{\beta}(c))), \sup_{c \in \overline{K+d}} (G_n^*(c) - n^r \sup_{b \in D} (\hat{\beta}(b) - \hat{\beta}(c)))) \leq x). \end{aligned} \quad (\text{A.12})$$

Let $L_n^*(x) = P^*(\sqrt{n}(\gamma_{\max, \text{modified}}^* - \hat{\gamma}_{\max}) \leq x)$. We notice that

$$n^r \sup_{c \in \overline{K+d}} \sup_{b \in D} (\hat{\beta}(b) - \hat{\beta}(c)) \leq n^r \sup_{c \in \overline{K+d}} \sup_{b \in D} (\hat{\beta}(b) - \beta(b) - (\hat{\beta}(c) - \beta(c))) - n^r \inf_{c \in \overline{K+d}} (\gamma_{\max} - \beta(c)). \quad (\text{A.13})$$

From Assumptions 4.1, 4.2 and 4.3, the 1st term of the right hand side of (A.13) converges to 0 in probability and the second term converges to negative infinite. Therefore, $n^r \sup_{b \in D} [\hat{\beta}(b) - \hat{\beta}(c)] \rightarrow -\infty$ uniformly for $c \in \overline{K+d}$ in probability and $L_n^*(x)$ is asymptotically equivalent to

$$P^* \left(\sup_{c \in K+d} (G_n^*(c) - n^r \sup_{b \in D} [\hat{\beta}(b) - \hat{\beta}(c)]) \leq x \right)$$

in probability. Similar to (A.13), we show that

$$\sup_{c \in K+d} |n^r \sup_{b \in D} [\hat{\beta}(b) - \hat{\beta}(c)] - n^r (\gamma_{\max} - \beta(c))| \rightarrow 0$$

in probability. Therefore, we have $L_n^*(x)$ is asymptotically equivalent to

$$P^* \left(\sup_{c \in K+d} (G_n^*(c) - n^r(\gamma_{\max} - \beta(c))) \leq x \right)$$

in probability. Now, we have the following inequality in probability.

$$P^* \left(\sup_{c \in K+d} G_n^*(c) \leq x \right) \leq \liminf L_n^*(x) \leq \limsup L_n^*(x) \leq P^* \left(\sup_{c \in K} G_n^*(c) \leq x \right).$$

With similar arguments used in the proof of Lemma 4.1 and Assumption 4.3, we prove the desired result. \square

Proof of Theorem 4: It naturally follows from Lemmas 4.1 and 4.2 with the property of the cdf. \square

With $\gamma_{\max} = \sup_c \beta(c)$, we let $S_n = \{c : \beta(c) \geq \gamma_{\max} - \log(n)/n\}$ and $\gamma_{ss} = \beta(\tilde{c})$, where \tilde{c} is a random variable as the value of c that achieves the minimum of $\beta(c)$ among all possible values of $\argmax_{c \in D} \hat{\beta}(c)$. We further denote the smallest value of c that achieves the maximum of $\beta(c)$, γ_{\max} , by c_0 , which is a well-defined fixed value from our continuous and compactness assumptions. Then, we have the following lemma to characterize the distribution of γ_{ss} .

Lemma 5.1: *Under Assumption 4.1, we have*

$$P(\gamma_{\max} - \gamma_{ss} \leq \log(n)/n) \rightarrow 1.$$

In other words, $P(\tilde{c} \in S_n) \rightarrow 1$, as $n \rightarrow \infty$.

Proof: If $\tilde{c} \notin S_n$, then, $\hat{\beta}(c_0) < \sup_{c \in \tilde{S}_n} \hat{\beta}(c)$. Therefore, we have,

$$\begin{aligned} & P(\gamma_{\max} - \gamma_{ss} > \log(n)/n) \\ & \leq P\left(\hat{\beta}(c_0) < \sup_{c \in \tilde{S}_n} \hat{\beta}(c)\right) \\ & = P\left(\sqrt{n}(\hat{\beta}(c_0) - \gamma_{\max}) < \sqrt{n} \sup_{c \in \tilde{S}_n} (\hat{\beta}(c) - \beta(c) + \beta(c) - \gamma_{\max})\right) \\ & \leq P\left(\sqrt{n}(\hat{\beta}(c_0) - \gamma_{\max}) < \sqrt{n} \sup_{c \in \tilde{S}_n} (\hat{\beta}(c) - \beta(c)) - \sqrt{n} \inf_{c \in \tilde{S}_n} (\gamma_{\max} - \beta(c))\right). \end{aligned} \tag{A.14}$$

Since $\sqrt{n} \sup_{c \in \tilde{S}_n} (\hat{\beta}(c) - \beta(c)) \leq \sqrt{n} \sup_{c \in D} (\hat{\beta}(c) - \beta(c))$ and $\sqrt{n} \inf_{c \in \tilde{S}_n} (\gamma_{\max} - \beta(c)) \geq \log(n)$, the right hand side of (A.14) converges to 0 and we finish the proof. \square

Lemma 5.2: *Under Assumption 4.1 and for any fixed x , we have*

$$P\left(\sqrt{n} \sup_{c \in S_n} (\hat{\beta}(c) - \beta(c)) \leq x\right) \rightarrow P(\sup_{c \in K} G(c) \leq x).$$

Proof: Since $S \subseteq S_n \subseteq S_2$, we can use similar techniques as those in the proof of Lemma 4.1. \square

Lemma 5.3: Let q_α be the $1 - \alpha$ quantile of $\sup_{c \in K} G(c)$, then, under Assumption 4.1, we have

$$\lim_{n \rightarrow \infty} P\left(\sqrt{n} \sup_{c \in D} (\hat{\beta}(c) - \gamma_{ss}) \leq q_\alpha\right) = 1 - \alpha.$$

Proof: From the definition, we know $\hat{\beta}(\tilde{c}) = \sup_{c \in D} \hat{\beta}(c)$ and $\gamma_{ss} = \beta(\tilde{c})$ so we have

$$\begin{aligned} & P\left(\sqrt{n} \sup_{c \in D} (\hat{\beta}(c) - \gamma_{ss}) \leq q_\alpha\right) \\ &= P\left(\sqrt{n} [\hat{\beta}(\tilde{c}) - \beta(\tilde{c})] (I_{\tilde{c} \in S_n} + I_{\tilde{c} \notin S_n}) \leq q_\alpha\right) \\ &= P\left(\sqrt{n} (\hat{\beta}(\tilde{c}) - \beta(\tilde{c})) \leq q_\alpha, \tilde{c} \in S_n\right) + P\left(\sqrt{n} (\hat{\beta}(\tilde{c}) - \beta(\tilde{c})) \leq q_\alpha, \tilde{c} \notin S_n\right). \end{aligned} \quad (\text{A.15})$$

From Lemma 5.1, we know the second part of the right hand side of (A.15) converges to 0. Notice that

$$\{\sqrt{n} (\hat{\beta}(\tilde{c}) - \beta(\tilde{c})) \leq q_\alpha, \tilde{c} \in S_n\} \supseteq \{\sqrt{n} \sup_{c \in S_n} ((\hat{\beta}(c) - \beta(c))) \leq q_\alpha, \tilde{c} \in S_n\},$$

from Lemmas 5.1 and 5.2, we have

$$\begin{aligned} & \liminf_{n \rightarrow \infty} P\left(\sqrt{n} (\hat{\beta}(\tilde{c}) - \beta(\tilde{c})) \leq q_\alpha, \tilde{c} \in S_n\right) \\ & \geq \liminf_{n \rightarrow \infty} P\left(\sqrt{n} \sup_{c \in S_n} ((\hat{\beta}(c) - \beta(c))) \leq q_\alpha, \tilde{c} \in S_n\right) \\ & = \liminf_{n \rightarrow \infty} P\left(\sqrt{n} \sup_{c \in S_n} ((\hat{\beta}(c) - \beta(c))) \leq q_\alpha\right) \rightarrow 1 - \alpha. \end{aligned} \quad (\text{A.16})$$

Since $\gamma_{ss} \leq \gamma_{\max} = \sup_{c \in D} \beta(c)$, from Lemma 4.1, we have

$$\limsup_{n \rightarrow \infty} P\left(\sqrt{n} \sup_{c \in D} (\hat{\beta}(c) - \gamma_{ss}) \leq q_\alpha\right) \leq \limsup_{n \rightarrow \infty} P\left(\sqrt{n} \sup_{c \in D} (\hat{\beta}(c) - \max_{c \in D} \beta(c)) \leq q_\alpha\right) = 1 - \alpha$$

Therefore, we complete the proof. \square

Proof of Theorem 5: It naturally follows from Lemma 5.3 and Theorem 4. \square

Appendix B

Synthetic Data of MONET1 Trial

To generate the synthetic data of the MONET1 trial, we consider a simple setting of n observations, $(Y_i, D_i, \delta_i, Z_i)$, $i = 1, \dots, n$, where Y_i is the (possibly censored) survival time of the i -th subject, D_i is the treatment indicator, δ_i is the censoring indicator, and $Z_i = (Z_{i,1}, \dots, Z_{i,K})$ is the subgroup indicator indicating whether the subject belongs to any of the $2K$ subgroups we consider.

Following the MONET1 trial in Kubota et al. (2014), we let $n = 1090$ and $K = 8$ with the following subgroups: East Asian patient or not ($Z_{i,1} = 1$ or 0), received radiotherapy or not ($Z_{i,2} = 1$ or 0), stage IIIB or not ($Z_{i,3} = 1$ or 0), Age greater than 65 or not ($Z_{i,4} = 1$ or 0), ECOG PS equal to 0 or not ($Z_{i,5} = 1$ or 0), Adenocarcinoma histology or not ($Z_{i,6} = 1$ or 0), male or female ($Z_{i,7} = 1$ or 0), and never smoked or not ($Z_{i,8} = 1$ or 0). We independently let $Z_{i,k} \sim \text{Bernoulli}(1, p_k)$, and $D_i \sim \text{Bernoulli}(1, p)$, where the parameters are estimated by the sample proportion in Table 1 and Figure 1.A in Kubota et al. (2014) and given in Table B.1. We independently generate the event time T_i by the distribution F and the censoring time C_i by the distribution G as defined in Table B.2, both of which are estimated based on Figure 1.A in Kubota et al. (2014) under the assumptions of no treatment effect. Finally, we obtain $Y_i = \min(T_i, C_i)$ and $\delta_i = I_{T_i \leq C_i}$.

Table B.1: Proportion of the subgroups p_i and the proportion p of subjects with treatment

p	p_1	p_2	p_3	p_4	p_5	p_6	p_7	p_8
0.5	0.208	0.143	0.139	0.339	0.362	0.817	0.615	0.281

Table B.2: Distribution for the event time and the censoring time: $F(x) = P(T = x)$ and $G(x) = P(C = x)$

x	8	16	24	32	40	48	56	64	72	80
F	0.05	0.05	0.08	0.06	0.06	0.06	0.04	0.05	0.03	0.04
G	0	0	0	0	0	1/15	1/15	1/15	1/15	1/15
x	88	96	104	112	120	128	136	144	152	160
F	0.04	0.04	0.02	0.02	0.02	0.02	0.02	0.00	0.00	0.3
G	0	0	0	0	2/15	2/15	2/15	2/15	2/15	0

Bibliography

Kubota, K et al. (2014). “Phase III study (MONET1) of motesanib plus carboplatin/paclitaxel in patients with advanced nonsquamous non-small-cell lung cancer (NSCLC): Asian subgroup analysis”. In: *Annals of oncology* 25(2), pp. 529–536.